updated CR

Test/civl/inductive-sequentialization/ChangRoberts.bpl
@@ -4,11 +4,9 @@
 const N: int; // size of the ring
 axiom N > 0;
 function {:inline} Next(i: int) : int { (i + 1) mod N }
-function {:inline} Prev(i: int) : int { (i - 1) mod N }
-
 function {:inline} ValidPid(pid: int) : bool { 0 <= pid && pid < N }
 
-var {:layer 0,4} leader: [int]bool;       // leader[pid] iff pid is a leader
+var {:layer 0,1} leader: [int]bool;       // leader[pid] iff pid is a leader
 
 // priority for becoming leader (ties are broken by pid)
 function Priority(int): int;      // pid -> priority
@@ -23,158 +21,36 @@ axiom ValidPid(ExpectedLeader);
 axiom (forall i: int:: ValidPid(i) ==> i == ExpectedLeader || Below(i, ExpectedLeader));
 
 // alternative coordinates for identifying processes where ExpectedLeader is at position 0
-// Pos converts from process id to its position
 // Pid converts from position to process id
-function {:inline} Pos(pid: int) : int { (pid - ExpectedLeader) mod N }
 function {:inline} Pid(pos: int) : int { (ExpectedLeader + pos) mod N }
 
 ////////////////////////////////////////////////////////////////////////////////
 
-function {:inline} Init(pids: [int]bool, leader: [int]bool) : bool
-{
-  pids == MapConst(true) &&
-  leader == MapConst(false)
-}
-
-////////////////////////////////////////////////////////////////////////////////
-
-atomic action {:layer 4} MAIN3(pids: Set int)
+yield left procedure {:layer 1} main()
+requires {:layer 1} leader == MapConst(false);
+ensures {:layer 1} leader == MapOne(ExpectedLeader);
 modifies leader;
 {
-  assert Init(pids->val, leader);
-  leader := MapConst(false)[ExpectedLeader := true];
-}
+  var pos: int;
+  var pid: int;
 
-action {:layer 3} INV2 (pids: Set int)
-creates P;
-modifies leader;
-{
-  /*
-  Invariant description:
-  
-  A (possibly empty) prefix of pending asyncs starting at position 0 is created.
-  The i-th pending async is created by process at position i and is targeted at 
-  the process at position Next(i).
-
-  A singleton pending async P(self, pid) is also created such that the position of
-  process pid is the length of the aforementioned prefix and self is a target whose
-  position is ahead of pid. This is the pending async chosen to be scheduled.
-  */
-  var {:pool "INV2"} choice: P; // nondeterministically chosen leading pending async
-  var self, pid: int;
-
-  assert Init(pids->val, leader);
-  assume {:add_to_pool "INV2", P(Next(choice->self), choice->pid), P(choice->pid, Prev(choice->pid))} true;
-  if (*) {
-    P(self, pid) := choice;
-    assume ValidPid(self) && ValidPid(pid);
-    // self is ahead of pid and may have wrapped around to position 0
-    assume Pos(self) == 0 || Pos(pid) < Pos(self);
-    // summarize the result of all priority comparisons by the leading pending async
-    // wraparound to position 0 is handled carefully
-    assume (forall {:pool "ORDER"} x: int :: {:add_to_pool "ORDER", x} Pos(pid) < x && x <= Prev(Pos(self)) ==> Below(Pid(x), pid));
-    // create prefix
-    call create_asyncs(
-      (lambda pa: P :: ValidPid(pa->pid) && Pos(pa->pid) < Pos(pid) && pa->self == Next(pa->pid)));
-    // create singleton and set the choice
-    async call P(self, pid);
-    call set_choice(choice);
-  } else {
-    leader[ExpectedLeader] := true;
-  }
-}
-////////////////////////////////////////////////////////////////////////////////
-
-atomic action {:layer 3} MAIN2(pids: Set int)
-refines MAIN3 using INV2;
-creates P;
-{
-  assert Init(pids->val, leader);
-  assume {:add_to_pool "INV2", P(ExpectedLeader, Prev(ExpectedLeader))} true;
-  call create_asyncs(
-    (lambda pa: P :: ValidPid(pa->pid) && pa->self == Next(pa->pid)));
-}
-
-action {:layer 2} INV1({:linear_in} pids: Set int)
-creates PInit, P;
-{
-  var {:pool "INV1"} k: int;
-  assert Init(pids->val, leader);
-
-  assume
-    {:add_to_pool "INV1", k+1}
-    {:add_to_pool "PInit", PInit(k)}
-    0 <= k && k <= N;
-  call create_asyncs((lambda {:pool "PInit"} pa: PInit :: k <= pa->self && pa->self < N));
-  call create_asyncs((lambda pa: P :: 0 <= pa->pid && pa->pid < k && pa->self == Next(pa->pid)));
-  call set_choice(PInit(k));
-}
-
-////////////////////////////////////////////////////////////////////////////////
-
-atomic action {:layer 2} MAIN1(pids: Set int)
-refines MAIN2 using INV1;
-creates PInit;
-{
-  assert Init(pids->val, leader);
-  assume {:add_to_pool "INV1", 0} true;
-  call create_asyncs((lambda pa: PInit :: ValidPid(pa->self)));
-}
-
-async left action {:layer 2} PInit(self: int)
-creates P;
-{
-  assert ValidPid(self);
-  async call P(Next(self), self);
-}
-
-async atomic action {:layer 2, 3} P(self: int, pid: int)
-creates P;
-modifies leader;
-{
-  assert ValidPid(self) && ValidPid(pid);
-  if (self == pid)
+  pos := N - 1;
+  while (0 <= pos)
+  invariant {:layer 1} pos < N;
+  invariant {:layer 1} if 0 <= pos then leader == MapConst(false) else leader == MapOne(ExpectedLeader);
   {
-    leader[pid] := true;
-  }
-  else if (Below(self, pid))
-  {
-    async call P(Next(self), pid);
+    pid := Pid(pos);
+    async call {:sync} p(Next(pid), pid);
+    pos := pos - 1;
   }
 }
 
-////////////////////////////////////////////////////////////////////////////////
-
-yield procedure {:layer 1} main(pids: Set int)
-refines MAIN1;
-{
-  var {:pending_async}{:layer 1} PAs: [PInit]int;
-  var pids': Set int;
-  var i: int;
-
-  pids' := pids;
-  i := 0;
-  while (i < N)
-  invariant {:layer 1} 0 <= i && i <= N;
-  invariant {:layer 1} (forall ii:int :: ValidPid(ii) && ii >= i ==> Set_Contains(pids', ii));
-  invariant {:layer 1} PAs == (lambda pa: PInit :: if ValidPid(pa->self) && pa->self < i then 1 else 0);
-  {
-    pids' := Set_Remove(pids', i);
-    async call pinit(i);
-    i := i + 1;
-  }
-}
-
-yield procedure {:layer 1} pinit(self: int)
-refines PInit;
-requires {:layer 1} ValidPid(self);
-{
-  async call p(Next(self), self);
-}
-
-yield procedure {:layer 1} p(self: int, pid: int)
-refines P;
+yield left procedure {:layer 1} p(self: int, pid: int)
 requires {:layer 1} ValidPid(self) && ValidPid(pid);
+requires {:layer 1} leader == MapConst(false);
+requires {:layer 1} pid == ExpectedLeader || (ExpectedLeader - self) mod N < (ExpectedLeader - pid) mod N;
+ensures {:layer 1} if pid == ExpectedLeader then leader == MapOne(ExpectedLeader) else leader == MapConst(false);
+modifies leader;
 {
   if (self == pid)
   {
@@ -182,16 +58,13 @@ requires {:layer 1} ValidPid(self) && ValidPid(pid);
   }
   else if (Below(self, pid))
   {
-    async call p(Next(self), pid);
+    async call {:sync} p(Next(self), pid);
   }
 }
 
 ////////////////////////////////////////////////////////////////////////////////
 
-both action {:layer 1} SET_LEADER(pid: int)
-modifies leader;
-{
+yield procedure {:layer 0} set_leader(pid: int);
+refines both action {:layer 1} _ {
   leader[pid] := true;
 }
-yield procedure {:layer 0} set_leader(pid: int);
-refines SET_LEADER;
